cvc5Test/Monadic.lean
@@ -1,0 +1,299 @@
+import cvc5
+
+
+
+namespace Cvc5.Term
+
+def mkAnd : (terms : Array Term) → Env Term := mk .AND
+def mkOr : (terms : Array Term) → Env Term := mk .OR
+
+def mk1 (op : cvc5.Kind) (term : Term) : Env Term := mk op #[term]
+def mk2 (op : cvc5.Kind) (lft rgt : Term) : Env Term := mk op #[lft, rgt]
+def mk3 (op : cvc5.Kind) (t1 t2 t3 : Term) : Env Term := mk op #[t1, t2, t3]
+
+def mkNot : Term → Env Term := mk1 .NOT
+
+def mkEq : Term → Term → Env Term := mk2 .EQUAL
+def mkLt : Term → Term → Env Term := mk2 .LT
+def mkLe : Term → Term → Env Term := mk2 .LEQ
+def mkEq0 (term : Term) : Env Term := mkInt 0 >>= mkEq term
+def mkLt0 (term : Term) : Env Term := mkInt 0 >>= mkLt term
+def mkLe0 (term : Term) : Env Term := mkInt 0 >>= mkLe term
+def mkAdd : Term → Term → Env Term := mk2 .ADD
+def mkSub : Term → Term → Env Term := mk2 .SUB
+def mkIte : Term → Term → Term → Env Term := mk3 .ITE
+
+end Cvc5.Term
+
+
+
+namespace Cvc5.Solver
+
+def check (assuming : Array Term := #[]) (solver : Solver) : Env Bool := do
+  let res ← solver.checkSatAssuming assuming
+  if res.isSat then return true
+  if res.isUnsat then return false
+  throw <| cvc5.Error.error s!"unexpected *unknown* check-sat result"
+
+end Cvc5.Solver
+
+
+
+namespace Test.Monadic
+
+open Cvc5 (EnvIO Term Solver Srt)
+
+
+
+structure TSys.Spec (SVars : Type) where
+  sVarsAt (k : Nat) : EnvIO SVars
+  sVarsToString : SVars → Array String
+  init : SVars → EnvIO Term
+  step : (curr : SVars) → (next : SVars) → EnvIO Term
+  getValues : Solver → SVars → EnvIO SVars
+  candidate : SVars → EnvIO Term
+
+inductive Result (SVars : Type)
+| safe (k : Nat) | cex (trace : Array SVars) | unknown
+
+namespace Result
+
+def isUnknown : Result SVars → Bool
+| .unknown => true | _ => false
+
+end Result
+
+structure TSys (SVars : Type) extends TSys.Spec SVars where private mk' ::
+  sVars : SVars × List SVars
+  baseSolver : Solver
+  stepSolver : Solver
+
+namespace TSys
+
+def mk (spec : Spec SVars) : EnvIO (TSys SVars) := do
+  let sVars0 ← spec.sVarsAt 0
+  let init0 ← spec.init sVars0
+  let baseSolver ← Solver.mk
+  baseSolver.setOption "produce-models" "true"
+  baseSolver.assert init0
+  let stepSolver ← Solver.mk
+  stepSolver.setOption "produce-models" "true"
+  let candidate0 ← spec.candidate sVars0
+  stepSolver.assert candidate0
+  return ⟨spec, (sVars0, []), baseSolver, stepSolver⟩
+
+def negCandidate (sVars : SVars) (sys : TSys SVars) : EnvIO Term := do
+  sys.candidate sVars >>= liftM ∘ Term.mkNot
+
+def currK (sys : TSys SVars) : Nat := sys.sVars.snd.length
+def currSVars (sys : TSys SVars) : SVars := sys.sVars.fst
+def allPreSVars (sys : TSys SVars) : List SVars := sys.sVars.snd
+def stageNextSVars (sys : TSys SVars) : EnvIO (SVars × TSys SVars) := do
+  let next ← sys.sVarsAt sys.currK.succ
+  let sVars := (next, sys.currSVars :: sys.allPreSVars)
+  return (next, {sys with sVars})
+
+abbrev Trace (_ : TSys SVars) := Array SVars
+abbrev Trace? (sys : TSys SVars) := Option sys.Trace
+protected abbrev Result (_ : TSys SVars) := Result SVars
+
+def printTrace (sys : TSys SVars) (trace : sys.Trace) (pref := "") : EnvIO Unit := do
+  let mut cnt := 0
+  let k := sys.currK
+  for sVars in trace do
+    let k := k - cnt
+    cnt := cnt + 1
+    let lines := sys.sVarsToString sVars
+    println! "{pref}- at {k}"
+    for line in lines do
+      println! "{pref}  {line}"
+
+def getCex (solver : Solver) (sys : TSys SVars) : EnvIO sys.Trace := do
+  let mut trace := Array.mkEmpty sys.sVars.snd.length
+  trace := trace.push (← sys.getValues solver sys.currSVars)
+  for sVars in sys.allPreSVars do
+    trace := trace.push (← sys.getValues solver sVars)
+  return trace
+
+def getBaseCex (sys : TSys SVars) : EnvIO sys.Trace :=
+  sys.getCex sys.baseSolver
+
+def getStepCex (sys : TSys SVars) : EnvIO sys.Trace :=
+  sys.getCex sys.stepSolver
+
+def getCex? (solver : Solver) (sys : TSys SVars)
+: EnvIO sys.Trace? := do
+  let bad ← sys.negCandidate sys.currSVars
+  let isSat ← solver.check #[bad]
+  if isSat then sys.getCex solver else return none
+
+def getBaseCex? (sys : TSys SVars) : EnvIO sys.Trace? := do
+  sys.getCex? sys.baseSolver
+
+def getStepCex? (sys : TSys SVars) : EnvIO sys.Trace? := do
+  sys.getCex? sys.stepSolver
+
+def unroll (sys : TSys SVars) : EnvIO (TSys SVars) := do
+  let curr := sys.currSVars
+  let currCandidate ← sys.candidate curr
+  let (next, sys) ← sys.stageNextSVars
+  let step ← sys.step curr next
+  sys.baseSolver.assert step
+  sys.stepSolver.assert currCandidate
+  sys.stepSolver.assert step
+  return sys
+
+def checkBaseUnrollCheckStep (sys : TSys SVars) : EnvIO (sys.Result × TSys SVars) := do
+  if let some baseCex ← sys.getBaseCex? then
+    return (.cex baseCex, sys)
+  else
+    let sys ← sys.unroll
+    if let some _stepCex ← sys.getStepCex? then
+      println! "step cex at {sys.currK}"
+      -- sys.printTrace stepCex
+      return (.unknown, sys)
+    else
+      return (.safe sys.currK, sys)
+
+
+def check' (sys : TSys SVars) : (maxK : Nat := 5) → EnvIO (sys.Result × TSys SVars)
+| 0 => return (.unknown, sys)
+| maxK + 1 => do
+  let (res, sys) ← sys.checkBaseUnrollCheckStep
+  if res.isUnknown then sys.check' maxK else return (res, sys)
+
+def check (sys : TSys SVars) (maxK : Nat := 5) : EnvIO sys.Result :=
+  Prod.fst <$> sys.check' maxK
+
+end TSys
+
+
+
+namespace Sw
+
+structure SVars where
+  startStop : Term
+  reset : Term
+  isCounting : Term
+  counter : Term
+
+def Spec (candidate : SVars → EnvIO Term) : TSys.Spec SVars where
+  sVarsAt k := do
+    let bool ← Srt.getBool
+    let int ← Srt.getInt
+    return ⟨
+      ← Cvc5.Term.mkConst s!"startStop@{k}" bool,
+      ← Cvc5.Term.mkConst s!"reset@{k}" bool,
+      ← Cvc5.Term.mkConst s!"isCounting@{k}" bool,
+      ← Cvc5.Term.mkConst s!"counter@{k}" int,
+    ⟩
+  getValues solver vars := return ⟨
+    ← solver.getValue vars.startStop,
+    ← solver.getValue vars.reset,
+    ← solver.getValue vars.isCounting,
+    ← solver.getValue vars.counter,
+  ⟩
+  sVarsToString vals := #[
+    s!"counter = {vals.counter}, isCounting = {vals.isCounting}",
+    s!"startStop = {vals.startStop}, reset = {vals.reset}",
+  ]
+  init vars := do
+    let notCounting ← vars.reset.mkNot
+    let counterGe0 ← (← Term.mkInt 0) |>.mkLe vars.counter
+    let init ← Term.mkAnd #[notCounting, counterGe0]
+    return init
+  step curr next := do
+    let isCountingDef ←
+      next.startStop.mkIte (← curr.isCounting.mkNot) curr.isCounting
+    let counterIncIfCounting ←
+      curr.counter.mkAdd (← next.isCounting.mkIte (← Term.mkInt 1) (← Term.mkInt 0))
+    let counterDef ←
+      next.reset.mkIte (← Term.mkInt 0) counterIncIfCounting
+    Term.mkAnd #[
+      ← next.isCounting.mkEq isCountingDef,
+      ← next.counter.mkEq counterDef,
+    ]
+  candidate
+
+def counterPos (vars : SVars) : EnvIO Term := do
+  (← Term.mkInt 0) |>.mkLe vars.counter
+
+def counterNotMinus7 (vars : SVars) : EnvIO Term := do
+  let eqM7 ← vars.counter.mkEq (← Term.mkInt (-7))
+  eqM7.mkNot
+
+def resetImpliesCounterIs0 (vars : SVars) : EnvIO Term := do
+  let notReset ← vars.reset.mkNot
+  let counterIs0 ← vars.counter.mkEq (← Term.mkInt 0)
+  Term.mkOr #[notReset, counterIs0]
+
+def allCandidates (vars : SVars) : EnvIO Term := do Term.mkAnd #[
+  ← counterPos vars,
+  ← counterNotMinus7 vars,
+  ← resetImpliesCounterIs0 vars,
+]
+
+def test' (candidate : SVars → EnvIO Term) : IO (Option Term) := Cvc5.Env.run do
+  let sys ← TSys.mk <| Sw.Spec candidate
+  let (res, sys) ← sys.check'
+  match res with
+  | .safe k =>
+    println! "candidate is {k}-inductive"
+    return ← sys.candidate sys.currSVars
+  | .cex trace =>
+    println! "found a counterexample"
+    sys.printTrace trace
+    return none
+  | .unknown =>
+    println! "could not reach a conclusion"
+    return none
+
+def test (candidate : SVars → EnvIO Term) : IO Unit := Cvc5.Env.run do
+  let _ ← test' candidate
+  return ()
+
+
+/-- info:
+candidate is 1-inductive
+-/
+#guard_msgs in #eval test counterPos
+
+/-- info:
+step cex at 1
+step cex at 2
+step cex at 3
+step cex at 4
+step cex at 5
+could not reach a conclusion
+-/
+#guard_msgs in #eval test counterNotMinus7
+
+/-- info:
+candidate is 1-inductive
+-/
+#guard_msgs in #eval test resetImpliesCounterIs0
+
+/-- info:
+candidate is 1-inductive
+-/
+#guard_msgs in #eval test allCandidates
+
+
+def run (candidate : SVars → EnvIO Term) : IO Unit := do
+  if let some invariant ← test' candidate then
+    let _ ← test fun vars => do
+      let other ← counterPos vars
+      Term.mkAnd #[invariant, other]
+  else println! "no invariant found"
+
+
+/-- info:
+candidate is 1-inductive
+error: cvc5.Error.error "invalid term in 'children' at index 0, expected a term associated with this term manager"
+error: cvc5.Error.error
+  "cvc5.Error.error \"invalid term in 'children' at index 0, expected a term associated with this term manager\""
+---
+error: cvc5.Error.error
+  "cvc5.Error.error \"invalid term in 'children' at index 0, expected a term associated with this term manager\""
+-/
+#guard_msgs in #eval run counterPos
